---
layout: post
title: Multiplying two 32-bit numbers without using 64-bit variable
---

In this post, we figure out how to multiplying two 32-bit positive numbers by only using 32-bit variables. Suppose that we are given two positive numbers $$x,y \in [0, 2^{32}-1]$$, the goal is to calculate $$z = x \times y$$ where $$z \in [0, 2^{64} - 1]$$ without using 64-bit any variable (and also, without using conditional expressions).

We use two variables, say $$z_1$$ and $$z_0$$, to represent $$z$$ where $$z_1$$ is 32 upper bits and $$z_0$$ is 32 lower bits of $$z$$, respectively. In other words, $$z = z_1 \times 2^{32} + z_0$$. So, our goal now is to find $$z_1$$ and $$z_0$$ using only calculations on 32-bit variables.

The first and naive idea is to decompose $$x$$ and $$y$$ into:

$$
x = x_1 \times 2^{16} + x_0,
$$

$$
y = y_1 \times 2^{16} + y_0,
$$

where $$x_0, x_1, y_0, y_1 \in [0, 2^{16}-1]$$ are 16-bit numbers. We then have:

$$
z = x_1y_1 \times 2^{32} + (x_0y_1 + x_1y_0) \times 2^{16} + x_0y_0
$$

When we see the factor $$2^{32}$$ here, we might say that let's take $$z_1 = x_1y_1$$ and $$z_0 = (x_0y_1 + x_1y_0) \times 2^{16} + x_0y_0$$ !?

Be careful! It is a bit more complicated than that. Why? Let's take a look on $$x_0y_0$$. Notice that $$x_0$$ and $$y_0$$ are 16-bit numbers. So their product is maximum 32 bits. It is similar to $$x_0y_1$$ and $$x_1y_0$$. Thus, $$(x_0y_1 + x_1y_0) \times 2^{16} + x_0y_0$$ does not fit 32 bits of $$z_0$$.

To deal with this, instead of considering two 32-bit parts $$z_1$$ and $$z_0$$, we consider $$z$$ as four 16-bit parts $$a_3, a_2, a_1, a_0 \in [0, 2^{16}-1]$$ such that:

$$
z = a_3 \times 2^{48} + a_2 \times 2^{32} + a_1 \times 2^{16} + a_0,
$$

or

$$
z_1 = a_3 \times 2^{16} + a_2,
$$

$$
z_0 = a_1 \times 2^{16} + a_0.
$$

Now we sequentially find $$a_0$$, $$a_1$$, $$a_2$$ and $$a_3$$. Before starting, we need to introduce the following two functions for a 32-bit number $$v$$:
- $$\mathsf{UP}(v)$$: returns the 16 upper bits of $$v$$,
- $$\mathsf{LO}(v)$$: returns the 16 lower bits of $$v$$.

Firstly, we start with $$a_0$$. Since only $$x_0y_0$$ involves in the value of $$a_0$$, it can be sure that $$a_0$$ is the lower 16 bits of $$x_0y_0$$. We write:

$$
a_0 = \mathsf{LO}(x_0y_0).
$$

Secondly, we find $$a_1$$. We have that $$x_0y_1$$, $$x_1y_0$$ and $$\mathsf{UP}(x_0y_0)$$ involve in the value of $$a_1$$. We need to calculate the sum of them and $$a_1$$ is the 16 lower bits of the sum. However, we have to be careful with the sum's calculation, otherwise, it can cause overflow. To have a closer look, we assign the maximum values for $$x_0, x_1, y_0, y_1$$. Namely,

$$
x_0 = x_1 = y_0 = y_1 = 65535 = (\texttt{FFFF})_{16},
$$

then

$$
x_0y_1 = x_1y_0 = 4294836225 = (\texttt{FFFE0001})_{16}
$$

We can observe that it is still possible to add $$2 \times \texttt{FFFF}$$ (twice of the maximum value of 16 bits) to $$x_0y_1$$ or $$x_1y_0$$ before it reaches the maximum value of 32 bits. Plus, we cannot calculate $$x_0y_1 + x_1y_0$$ directly. So, we do the following steps:

$$
a_1 = \mathsf{LO}(x_1y_0 + \mathsf{LO}(x_0y_1 + \mathsf{UP}(x_0y_0)))
$$

Thirdly, we find $$a_2$$. We have that $$x_1y_1$$ and all the calculations before ($$x_0y_1$$, $$x_1y_0$$ and $$\mathsf{UP}(x_0y_0)$$) involve in the value of $$a_2$$ (in case their sums are propagatedly over 16 bits). We pay attention to the calculations before in $$a_1$$ where we only take the lower bits, including $$x_0y_1 + \mathsf{UP}(x_0y_0)$$ and $$x_1y_0 + \mathsf{LO}(x_0y_1 + \mathsf{UP}(x_0y_0))$$. Now:

$$
\begin{align}
a_2 = \mathsf{LO}   &( \\
                    &x_1y_1 + \\ 
                    &\mathsf{UP}(x_0y_1 + \mathsf{UP}(x_0y_0)) + \\
                    &\mathsf{UP}(x_1y_0 + \mathsf{LO}(x_0y_1 + \mathsf{UP}(x_0y_0))) \\
                    &)
\end{align}
$$

Finally, we find $$a_3$$. It is similar to $$a_2$$, but we take the upper bits at the end:

$$
\begin{align}
a_3 = \mathsf{UP}   &( \\
                    &x_1y_1 + \\ 
                    &\mathsf{UP}(x_0y_1 + \mathsf{UP}(x_0y_0)) + \\
                    &\mathsf{UP}(x_1y_0 + \mathsf{LO}(x_0y_1 + \mathsf{UP}(x_0y_0))) \\
                    &)
\end{align}
$$

NOTE: It is not necessary to calculate $$a_2$$ and $$a_3$$ separately, because:

$$
z_1 = a_3 \times 2^{16} + a_2 = x_1y_1 + \mathsf{UP}(x_0y_1 + \mathsf{UP}(x_0y_0)) + \mathsf{UP}(x_1y_0 + \mathsf{LO}(x_0y_1 + \mathsf{UP}(x_0y_0))))
$$

VoilÃ . Now we have
$$
z_1 = a_3 \times 2^{16} + a_2
$$
and
$$
z_0 = a_1 \times 2^{16} + a_0.
$$
Below is the C implementation and here is the link to github: [https://github.com/nvietsang/mult32](https://github.com/nvietsang/mult32)

```
#define UP(x) (x >> 16)      // 16 upper bits
#define LO(x) (x & 0xFFFF)   // 16 lower bits

/**
 * Given:
 *  x = x1 * 2^16 + x0
 *  y = y1 * 2^16 + y0
 * Compute:
 *  z = x * y
 * Return:
 *  z[1]: 32 upper bits
 *  z[0]: 32 lower bits
*/
void mult32(unsigned int *z, unsigned int x, unsigned int y) {
	unsigned int x1 = UP(x);
	unsigned int x0 = LO(x);
	unsigned int y1 = UP(y);
	unsigned int y0 = LO(y);

    unsigned int t;
    // z = z3 * 2^48 + z2 * 2^32 + z1 * 2^16 + z0
    // z[1] = z3 * 2^16 + z2 
    // z[0] = z1 * 2^16 + z0
    unsigned int z3, z2, z1, z0; 
    t = x0 * y0;
    z0 = LO(t);
    
    z1 = UP(t);
    t = x0 * y1 + z1;
    z1 = LO(t);
    z2 = UP(t);

    t = x1 * y0 + z1;
    z1 = LO(t);
    z2 = UP(t) + z2;
    t = x1 * y1 + z2;
    // z2 = LO(t);
    // z3 = UP(t);
    
    z[1] = t;
    // z[1] = (z3 << 16) | z2;
    z[0] = (z1 << 16) | z0;
}

```